Still broken but FINITE_rule results are proved.
Unfortunately, they require that the input alphabet be finite.

pda/homomorphismScript.sml
@@ -13,8 +13,6 @@ open gnfTheory
 val _ = new_theory "homomorphism"
 
 
-val _ = Globals.linewidth := 60
-val _ = set_trace "Unicode" 1
 val _ = diminish_srw_ss ["list EQ"];
 
 val stkSymsInPda = Define
@@ -39,7 +37,7 @@ METIS_TAC [mem_in]);
 
 val stkSymsPdaInv = store_thm
 ("stkSymsPdaInv",
-``∀x y.(ID m)^* x y ⇒ 
+``∀x y.(ID m)^* x y ⇒
 ∀q i s.(x=(q,i,s)) ⇒ (y=(q',i',s')) ⇒ stkSymsInPda m s
 ⇒
 stkSymsInPda m s'``,
@@ -53,7 +51,7 @@ FULL_SIMP_TAC (srw_ss()) [stkSymsInPda] THEN
 SRW_TAC [][] THEN
 `sh ∈ stkSyms m` by (FULL_SIMP_TAC (srw_ss()) [stkSyms_def, EXTENSION] THEN
  METIS_TAC []) THEN
- `∀e.MEM e st' ⇒  e ∈ stkSyms m` 
+ `∀e.MEM e st' ⇒  e ∈ stkSyms m`
  by METIS_TAC [memStkSyms] THEN
 METIS_TAC []);
 
@@ -85,7 +83,7 @@ val idcStkNil' = store_thm
 ``∀x y.(ID m)^* x y ⇒ (x=(q,i,[])) ⇒ (y=(q,i,[]))``,
 
 HO_MATCH_MP_TAC RTC_STRONG_INDUCT THEN SRW_TAC [][] THEN
-Cases_on `x'` THEN 
+Cases_on `x'` THEN
 Cases_on `r` THEN
 FULL_SIMP_TAC (srw_ss()) [id_thm]);
 
@@ -118,31 +116,31 @@ SRW_TAC [][listderiv_def] THEN1
 METIS_TAC [rtc2list_distrib_append_fst] THEN1
 (Cases_on `l` THEN FULL_SIMP_TAC (srw_ss()) []) THEN
 `l=FRONT l ++ [LAST l]` by METIS_TAC [APPEND_FRONT_LAST] THEN
-`rtc2list R ([LAST l]++[e])` 
+`rtc2list R ([LAST l]++[e])`
  by METIS_TAC [MEM, MEM_APPEND, rtc2list_distrib_append_snd, APPEND_ASSOC] THEN
 FULL_SIMP_TAC (srw_ss()) []);
 
 
 val rule1 = Define
-`rule1 m h = 
-{ ((NONE,ssym,q,x),(p,x),ssyms) | ∃a. isSuffix x (h a) ∧ 
+`rule1 (m:(α, β, γ) pda) (h: α -> α list) =
+{ ((NONE:α option,ssym,q,x),(p,x),ssyms) | ∃a. isSuffix x (h a) ∧
  MEM ((NONE,ssym,q),(p,ssyms)) m.next }`;
 
 val rule2 = Define
-`rule2 m h =
-{ ((NONE,ssym,(q,isym::x)),((p,x),ssyms)) | ∃a. isSuffix (isym::x) (h a) ∧ 
+`rule2 (m:(α, β, γ) pda) (h: α -> α list) =
+{ ((NONE:α option,ssym,(q,isym::x)),((p,x),ssyms)) | ∃a. isSuffix (isym::x) (h a) ∧
 MEM ((SOME isym,ssym,q),(p,ssyms)) m.next }`;
 
 val rule3 = Define
 `rule3 (m:(α, β, γ) pda) (h: α -> α list) newssym=
-{ ((SOME a,ssym,(q,[])),((q,h a),[ssym])) | a,ssym,q |
+{ ((SOME a,ssym,(q,[]:α list)),((q,h a),[ssym])) | a,ssym,q |
 q ∈ states m ∧ ssym ∈ (stkSyms m ∪ {newssym}) ∧ (h a) ∈ IMAGE h {a} }`;
 
 
 val hInvpda = Define
-`hInvpda (m:(α, β, γ) pda) (m':(α, β, γ # α list) pda) (h: α -> α list) = 
-∃z0. z0 ∉ stkSyms m ∧ (m'.ssSym = z0) ∧ 
-∃q0. q0 ∉ states m ∧ (m'.start = (q0,[]:α list)) ∧ 
+`hInvpda (m:(α, β, γ) pda) (m':(α, β, γ # α list) pda) (h: α -> α list) =
+∃z0. z0 ∉ stkSyms m ∧ (m'.ssSym = z0) ∧
+∃q0. q0 ∉ states m ∧ (m'.start = (q0,[]:α list)) ∧
 (∀q r.MEM (q,r:α list) m'.final = MEM q m.final ∧ (r=[])) ∧
 ∀r.MEM r m'.next = r ∈ (rule1 m h ∪ rule2 m h ∪ rule3 m h m'.ssSym) ∪
 { ((NONE,m'.ssSym,m'.start),((m.start,[]),[m.ssSym;m'.ssSym])) } `;
@@ -169,11 +167,11 @@ val mImpm'Trans1 = store_thm
 `MEM ((NONE,sh,q,h a),(p,h a),st') m'.next`
  by METIS_TAC [memMRule1, isSuffix_refl] THEN
  SRW_TAC [][Once RTC_CASES1] THEN
- `q ∈ states m` by 
+ `q ∈ states m` by
  (SRW_TAC [][states_def, EXTENSION] THEN
   METIS_TAC []) THEN
  `sh ∈ stkSyms m'` by (SRW_TAC [][stkSyms_def, EXTENSION] THEN METIS_TAC []) THEN
- `MEM ((SOME a,sh,q,[]),(q,h a),[sh]) m'.next` 
+ `MEM ((SOME a,sh,q,[]),(q,h a),[sh]) m'.next`
  by (FULL_SIMP_TAC (srw_ss()) [rule3, hInvpda] THEN
      FULL_SIMP_TAC (srw_ss()) [rule2,rule3]  THEN
      RES_TAC THEN FULL_SIMP_TAC (srw_ss()) [] THEN SRW_TAC [][] THEN
@@ -184,7 +182,7 @@ val mImpm'Trans1 = store_thm
 
 val mImpm'Trans2 = store_thm
 ("mImpm'Trans2",
-``MEM ((SOME ih,sh,q),p,st') m.next ∧ (h a = ih::isyms) ∧ hInvpda m m' h 
+``MEM ((SOME ih,sh,q),p,st') m.next ∧ (h a = ih::isyms) ∧ hInvpda m m' h
  ⇒
 IDC m' ((q,[]),[a],sh::st) ((p,isyms),[],st' ++ st)``,
 
@@ -195,8 +193,8 @@ IDC m' ((q,[]),[a],sh::st) ((p,isyms),[],st' ++ st)``,
      METIS_TAC [isSuffix_lemma,APPEND]) THEN
  `q ∈ states m` by (SRW_TAC [][states_def, EXTENSION] THEN METIS_TAC []) THEN
  `sh ∈ stkSyms m'` by (SRW_TAC [][stkSyms_def, EXTENSION] THEN METIS_TAC []) THEN
- `MEM ((SOME a,sh,q,[]),(q,h a),[sh]) m'.next` 
- by (FULL_SIMP_TAC (srw_ss()) [hInvpda, rule3] THEN 
+ `MEM ((SOME a,sh,q,[]),(q,h a),[sh]) m'.next`
+ by (FULL_SIMP_TAC (srw_ss()) [hInvpda, rule3] THEN
      FULL_SIMP_TAC (srw_ss()) [rule1,rule3]  THEN
      RES_TAC THEN FULL_SIMP_TAC (srw_ss()) [] THEN SRW_TAC [][] THEN
      METIS_TAC [memStkSyms]) THEN
@@ -209,9 +207,9 @@ IDC m' ((q,[]),[a],sh::st) ((p,isyms),[],st' ++ st)``,
 
 val mImpm'OneSym = store_thm
 ("mImpm'OneSym",
-``∀dl p isyms ssyms'.ID m ⊢ dl ◁ (q,h a,ssyms) → (p,isyms,ssyms') ∧ 
+``∀dl p isyms ssyms'.ID m ⊢ dl ◁ (q,h a,ssyms) → (p,isyms,ssyms') ∧
 LENGTH dl > 1 ∧
-hInvpda (m:(α, β, γ) pda) (m':(α, β, γ # α list) pda) (h: α -> α list) 
+hInvpda (m:(α, β, γ) pda) (m':(α, β, γ # α list) pda) (h: α -> α list)
 ⇒
  IDC m' ((q,[]),[a],ssyms) ((p,isyms),[],ssyms')``,
 
@@ -236,11 +234,11 @@ FULL_SIMP_TAC (srw_ss()) [id_thm] THEN
 SRW_TAC [][] THEN
 RES_TAC
 THENL[
-      `isSuffix isyms (h a)` by METIS_TAC [APPEND, isSuffix_APPEND, 
+      `isSuffix isyms (h a)` by METIS_TAC [APPEND, isSuffix_APPEND,
 					   idcInpSplit] THEN
       IMP_RES_TAC memMRule1 THEN
       `MEM ((NONE,sh,q',isyms),(p,isyms),st') m'.next`
-      by (FULL_SIMP_TAC (srw_ss()) [rule2, hInvpda] THEN 
+      by (FULL_SIMP_TAC (srw_ss()) [rule2, hInvpda] THEN
 	  METIS_TAC [APPEND, isSuffix_lemma]) THEN
       `ID m' ((q',isyms),[],sh::st) ((p,isyms),[],st' ++ st)`
       by SRW_TAC [][id_thm] THEN
@@ -248,10 +246,10 @@ THENL[
 
       `isSuffix (ih::isyms) (h a)` by METIS_TAC [APPEND, isSuffix_APPEND,
 						 idcInpSplit] THEN
-      `isSuffix isyms (h a)` by 
+      `isSuffix isyms (h a)` by
       METIS_TAC [isSuffix_APPEND, APPEND, APPEND_ASSOC] THEN
       `MEM ((NONE,sh,q',ih::isyms),(p,isyms),st') m'.next`
-      by (FULL_SIMP_TAC (srw_ss()) [rule2, hInvpda] THEN 
+      by (FULL_SIMP_TAC (srw_ss()) [rule2, hInvpda] THEN
 	  METIS_TAC [isSuffix_lemma, APPEND]) THEN
       `ID m' ((q',ih::isyms),[],sh::st) ((p,isyms),[],st' ++ st)`
       by SRW_TAC [][id_thm] THEN
@@ -261,7 +259,7 @@ THENL[
 val mImpm'InpNil = store_thm
 ("mImpm'InpNil",
 ``∀dl q ssyms p.
-ID m ⊢ dl ◁ (q,[],ssyms) → (p,[],ssyms') ∧ hInvpda m m' h 
+ID m ⊢ dl ◁ (q,[],ssyms) → (p,[],ssyms') ∧ hInvpda m m' h
  ⇒
 IDC m' ((q,[]),[],ssyms) ((p,[]),[],ssyms')``,
 
@@ -285,7 +283,7 @@ METIS_TAC [RTC_RULES]);
 val idTransOnInpPfx = store_thm
 ("idTransOnInpPfx",
 ``∀q x y ssyms.
-      ID m ⊢ dl ◁ (q,x++y,ssyms) → (p,[],ssyms') 
+      ID m ⊢ dl ◁ (q,x++y,ssyms) → (p,[],ssyms')
       ⇒
       ∃q0 ssyms0.
       IDC m (q,x++y,ssyms) (q0,y,ssyms0) ∧ IDC m (q0,y,ssyms0) (p,[],ssyms')``,
@@ -295,7 +293,7 @@ Cases_on `dl` THEN FULL_SIMP_TAC (srw_ss()) [listderiv_def] THEN
 SRW_TAC [][] THEN1
 METIS_TAC [APPEND_NIL,  RTC_RULES] THEN
 Cases_on `h'` THEN Cases_on `r` THEN
-FULL_SIMP_TAC (srw_ss()) [id_thm] THEN SRW_TAC [][] 
+FULL_SIMP_TAC (srw_ss()) [id_thm] THEN SRW_TAC [][]
 THENL[
       FIRST_X_ASSUM (Q.SPECL_THEN [`x`,`y`] MP_TAC) THEN SRW_TAC [][] THEN
       FULL_SIMP_TAC (srw_ss()) [] THEN
@@ -312,12 +310,12 @@ THENL[
 	    Q.EXISTS_TAC `q` THEN
 	    Q.EXISTS_TAC `sh::st` THEN
 	    SRW_TAC [][] THEN
-	    `ID m (q,ih::(x++y),sh::st) (q',(x++y),st'++st)` 
+	    `ID m (q,ih::(x++y),sh::st) (q',(x++y),st'++st)`
 	    by SRW_TAC [][id_thm] THEN
 	    METIS_TAC [RTC_RULES, RTC_RTC],
 
 	    FIRST_X_ASSUM (Q.SPECL_THEN [`t'`,`y`] MP_TAC) THEN SRW_TAC [][] THEN
-	    `ID m (q,h::(t' ++ y),sh::st) (q',t' ++ y,st' ++ st)` 
+	    `ID m (q,h::(t' ++ y),sh::st) (q',t' ++ y,st' ++ st)`
 	    by SRW_TAC [][id_thm] THEN
 	    METIS_TAC [RTC_RULES]
 	    ]]);
@@ -381,14 +379,14 @@ METIS_TAC [mem_in]);
 val m'toBufInpNil = store_thm
 ("m'toBufInpNil",
 ``∀dl q ssyms.
-ID m' ⊢ dl ◁ ((q,[]),[],ssyms) → ((p,r),[],ssyms') ⇒ hInvpda m m' h 
+ID m' ⊢ dl ◁ ((q,[]),[],ssyms) → ((p,r),[],ssyms') ⇒ hInvpda m m' h
 ⇒
 (r=[])``,
 
 Induct_on `dl` THEN SRW_TAC [][] THEN1
 FULL_SIMP_TAC (srw_ss()) [listderiv_def] THEN
 Cases_on `dl` THEN1 (FULL_SIMP_TAC (srw_ss()) [listderiv_def] THEN SRW_TAC [][]) THEN
-IMP_RES_TAC listDerivHdBrk THEN 
+IMP_RES_TAC listDerivHdBrk THEN
 `h'=((q,[]),[],ssyms)`by FULL_SIMP_TAC (srw_ss()) [listderiv_def] THEN
 SRW_TAC [][] THEN
 Cases_on `h''` THEN
@@ -414,7 +412,7 @@ ID m' ⊢ dl ◁ ((q,[]),[e],ssyms) → ((p,r),[],ssyms') ∧ hInvpda m m' h  �
 Induct_on `dl` THEN SRW_TAC [][] THEN1
 FULL_SIMP_TAC (srw_ss()) [listderiv_def] THEN
 Cases_on `dl` THEN1 (FULL_SIMP_TAC (srw_ss()) [listderiv_def] THEN SRW_TAC [][]) THEN
-IMP_RES_TAC listDerivHdBrk THEN 
+IMP_RES_TAC listDerivHdBrk THEN
 `h'=((q,[]),[e],ssyms)`by FULL_SIMP_TAC (srw_ss()) [listderiv_def] THEN
 SRW_TAC [][] THEN
 Cases_on `h''` THEN
@@ -429,10 +427,10 @@ FULL_SIMP_TAC (srw_ss()) [] THEN SRW_TAC [][] THEN1
  SRW_TAC [][] THEN
  RES_TAC THEN
  FULL_SIMP_TAC (srw_ss()) [] THEN SRW_TAC [][] THEN
- `hInvpda m m' h ` by FULL_SIMP_TAC (srw_ss()) [hInvpda, rule1, rule2, rule3, 
+ `hInvpda m m' h ` by FULL_SIMP_TAC (srw_ss()) [hInvpda, rule1, rule2, rule3,
 						  EXTENSION] THEN
  METIS_TAC [m'toBufInpNil]) THEN
-`hInvpda m m' h` by FULL_SIMP_TAC (srw_ss()) [hInvpda, rule1, rule2, rule3, 
+`hInvpda m m' h` by FULL_SIMP_TAC (srw_ss()) [hInvpda, rule1, rule2, rule3,
 						 EXTENSION] THEN
 METIS_TAC [m'toBufInpNil]);
 
@@ -440,16 +438,16 @@ METIS_TAC [m'toBufInpNil]);
 
 val m'Rule1 = store_thm
 ("m'Rule1",
-``MEM ((NONE,sh,q,[]),(q'',r),st') m'.next ∧ hInvpda m m' h 
+``MEM ((NONE,sh,q,[]),(q'',r),st') m'.next ∧ hInvpda m m' h
 ⇒
 (r=[])``,
 
 SRW_TAC [][hInvpda] THEN
 `∀a.isSuffix [] (h a)` by SRW_TAC [][isSuffix_def] THEN
 FULL_SIMP_TAC (srw_ss()) [rule1, rule2, rule3] THEN
-Q.PAT_ASSUM `∀e.P` MP_TAC THEN 
-Q.PAT_ASSUM `∀e.P` MP_TAC THEN 
-FIRST_X_ASSUM (Q.SPECL_THEN [`((NONE,sh,q,[]),(q'',r),st')`] MP_TAC) THEN 
+Q.PAT_ASSUM `∀e.P` MP_TAC THEN
+Q.PAT_ASSUM `∀e.P` MP_TAC THEN
+FIRST_X_ASSUM (Q.SPECL_THEN [`((NONE,sh,q,[]),(q'',r),st')`] MP_TAC) THEN
 SRW_TAC [][] THEN
 METIS_TAC []);
 
@@ -465,7 +463,7 @@ Cases_on `x'` THEN
 Cases_on `r` THEN
 FULL_SIMP_TAC (srw_ss()) [id_thm] THEN SRW_TAC [][]
 THENL[
-      Cases_on `st` THEN FULL_SIMP_TAC (srw_ss()) [] 
+      Cases_on `st` THEN FULL_SIMP_TAC (srw_ss()) []
       THENL[
 	    Cases_on `LENGTH st' > 0` THEN FULL_SIMP_TAC (srw_ss()) [] THEN
 	    SRW_TAC [][]
@@ -492,12 +490,12 @@ THENL[
 
 	    FULL_SIMP_TAC (arith_ss) [] THEN
 	    SRW_TAC [][] THEN
-	    (`ID m (q,i,sh::h::t) (q'',i,st' ++ h::t)` 
+	    (`ID m (q,i,sh::h::t) (q'',i,st' ++ h::t)`
 	     by SRW_TAC [][id_thm] THEN
 	     METIS_TAC [RTC_RULES])
 	    ],
 
-      Cases_on `st` THEN FULL_SIMP_TAC (srw_ss()) [] 
+      Cases_on `st` THEN FULL_SIMP_TAC (srw_ss()) []
       THENL[
 	    Cases_on `LENGTH st' > 0` THEN FULL_SIMP_TAC (srw_ss()) [] THEN
 	    SRW_TAC [][]
@@ -523,7 +521,7 @@ THENL[
 
 	    FULL_SIMP_TAC (arith_ss) [] THEN
 	    SRW_TAC [][] THEN
-	    (`ID m (q,ih::q''',sh::h::t) (q'',q''',st' ++ h::t)` 
+	    (`ID m (q,ih::q''',sh::h::t) (q'',q''',st' ++ h::t)`
 	     by SRW_TAC [][id_thm] THEN
 	     METIS_TAC [RTC_RULES])
 	    ]]);
@@ -535,7 +533,7 @@ val memStates = store_thm
  ⇒
 q ∈ states m ∧ q' ∈ states m``,
 
-Induct_on `dl` THEN SRW_TAC [][] 
+Induct_on `dl` THEN SRW_TAC [][]
 THENL[
       Cases_on `dl` THEN FULL_SIMP_TAC (srw_ss()) [listderiv_def] THEN
       SRW_TAC [][] THEN
@@ -544,7 +542,7 @@ THENL[
       SRW_TAC [][] THEN
       FULL_SIMP_TAC (srw_ss()) [states_def, EXTENSION] THEN
       METIS_TAC [],
-      
+
       Cases_on `dl` THEN FULL_SIMP_TAC (srw_ss()) [listderiv_def] THEN
       SRW_TAC [][] THEN
       Cases_on `h'` THEN
@@ -559,7 +557,7 @@ THENL[
 
 val idZ0Inv = store_thm
 ("idZ0Inv",
-``m' ⊢ (q,i,p ++ [m'.ssSym]) → (q0,i0,s0) ∧ hInvpda m m' h 
+``m' ⊢ (q,i,p ++ [m'.ssSym]) → (q0,i0,s0) ∧ hInvpda m m' h
 ⇒
 ∃pfx. s0 = pfx ++ [m'.ssSym]``,
 
@@ -570,7 +568,7 @@ FULL_SIMP_TAC (srw_ss()) [hInvpda, rule1, rule2,rule3, EXTENSION] THEN
 IMP_RES_TAC twoListAppEq THEN SRW_TAC [][] THEN
 FULL_SIMP_TAC (srw_ss()) [] THEN SRW_TAC [][] THEN
 (Cases_on `p` THEN SRW_TAC [][] THEN
- FULL_SIMP_TAC (srw_ss()) [] THEN 
+ FULL_SIMP_TAC (srw_ss()) [] THEN
  SRW_TAC [][] THEN
 Cases_on `s2` THEN FULL_SIMP_TAC (srw_ss()) [] THEN
 SRW_TAC [][] THEN
@@ -579,29 +577,29 @@ SRW_TAC [][] THEN
 val z0Inv = store_thm
 ("z0Inv",
 ``∀dl q i s p.ID m' ⊢ dl ◁ (q,i,s) → (q',i',s') ∧ hInvpda m m' h  ∧
-(s=p++[m'.ssSym]) 
+(s=p++[m'.ssSym])
 ⇒
 (∀q0 i0 s0.MEM (q0,i0,s0) dl ⇒ ∃pfx.(s0 = pfx++[m'.ssSym]))``,
 
-Induct_on `dl` THEN SRW_TAC [][] 
+Induct_on `dl` THEN SRW_TAC [][]
 THENL[
       Cases_on `dl` THEN FULL_SIMP_TAC (srw_ss()) []  THEN
       FULL_SIMP_TAC (srw_ss()) [listderiv_def] THEN
       SRW_TAC [][],
-      
+
       Cases_on `dl` THEN FULL_SIMP_TAC (srw_ss()) [] THEN
-      SRW_TAC [][] 
+      SRW_TAC [][]
       THENL[
 	    FULL_SIMP_TAC (srw_ss()) [listderiv_def] THEN
 	    SRW_TAC [][] THEN
 	    METIS_TAC [idZ0Inv],
 
 	    IMP_RES_TAC listDerivHdBrk THEN
-	    `h' = ((q,i,p ++ [m'.ssSym]))` 
+	    `h' = ((q,i,p ++ [m'.ssSym]))`
 	    by FULL_SIMP_TAC (srw_ss()) [listderiv_def] THEN
 	    SRW_TAC [][] THEN
 	    Cases_on `h''` THEN
-	    Cases_on `r` THEN	    
+	    Cases_on `r` THEN
 	    IMP_RES_TAC idZ0Inv THEN
 	    SRW_TAC [][] THEN
 	    METIS_TAC []]]);
@@ -609,8 +607,8 @@ THENL[
 
 val memStkSymsEq = store_thm
 ("memStkSymsEq",
-``e ∈ stkSyms m = (e=m.ssSym) ∨ 
-∃io ssym q q' ssyms.(MEM ((io,ssym,q),q',ssyms) m.next ∧ 
+``e ∈ stkSyms m = (e=m.ssSym) ∨
+∃io ssym q q' ssyms.(MEM ((io,ssym,q),q',ssyms) m.next ∧
 		      ((e=ssym) ∨ MEM e ssyms))``,
 
 SRW_TAC [][stkSyms_def, EXTENSION, EQ_IMP_THM] THEN1
@@ -642,7 +640,7 @@ Cases_on `l1` THEN FULL_SIMP_TAC (srw_ss()) [] THEN
 FIRST_X_ASSUM (Q.SPECL_THEN [`t`] MP_TAC) THEN SRW_TAC [][] THEN
 SRW_TAC [][ Once RTC_CASES1] THEN
  FULL_SIMP_TAC (srw_ss()) [id_thm, hInvpda, rule3, EXTENSION,rule1,rule2] THEN
- Cases_on `s` THEN FULL_SIMP_TAC (srw_ss()) [] 
+ Cases_on `s` THEN FULL_SIMP_TAC (srw_ss()) []
  THENL[
        Q.EXISTS_TAC `((q,[]),t,[m'.ssSym])` THEN
        SRW_TAC [][id_thm] THEN
@@ -653,7 +651,7 @@ SRW_TAC [][ Once RTC_CASES1] THEN
        Q.EXISTS_TAC `((q,[]),t,h''::(t'++[m'.ssSym]))` THEN
        SRW_TAC [][id_thm] THEN
        FULL_SIMP_TAC (srw_ss()) [] THEN
-       `hInvpda m m' h` 
+       `hInvpda m m' h`
        by FULL_SIMP_TAC (srw_ss()) [rule1,rule2,rule3,EXTENSION,hInvpda] THEN
        METIS_TAC [ stkSymsInPda,stkSymsPdaInv,MEM,memStkSyms,
 		  memStksymsm']
@@ -684,7 +682,7 @@ METIS_TAC [memStkSymsEq]);
 
 val stkSymsm'Impm = store_thm
 ("stkSymsm'Impm",
-``stkSymsInPda m' l ∧ hInvpda m m' h ⇒ 
+``stkSymsInPda m' l ∧ hInvpda m m' h ⇒
 (∀e.MEM e l ⇒ e ∈ stkSyms m ∨ (e=m'.ssSym))``,
 
 Induct_on `l` THEN SRW_TAC [][] THEN
@@ -720,20 +718,20 @@ Induct_on `LENGTH x` THEN SRW_TAC [][] THEN1
  `∃l.ID m ⊢ l ◁ (q,h h' ++ FLAT (MAP h t),ssyms) → (q0,FLAT (MAP h t),ssyms0)`
  by METIS_TAC [rtc2list_exists'] THEN
  IMP_RES_TAC idTransOnInpPfxToNil THEN
- `∃l'.ID m ⊢ l' ◁ (q,h h',ssyms) → (q0,[],ssyms0)` 
+ `∃l'.ID m ⊢ l' ◁ (q,h h',ssyms) → (q0,[],ssyms0)`
  by METIS_TAC [rtc2list_exists', memld,z0Inv] THEN
  Cases_on `LENGTH l' > 1`
 THENL[
       IMP_RES_TAC mImpm'OneSym THEN
-      `(ID m')^* ((q,[]),[h'],ssyms) ((q0,[]),[],ssyms0)` 
+      `(ID m')^* ((q,[]),[h'],ssyms) ((q0,[]),[],ssyms0)`
       by METIS_TAC [rtc2list_exists'] THEN
       `∃dl'.ID m ⊢ dl' ◁ (q0,FLAT (MAP h t),ssyms0) → (p,[],ssyms')`
       by METIS_TAC [rtc2list_exists'] THEN
       Cases_on `LENGTH dl' > 1` THEN1
-      (`(ID m')^* ((q,[]),[h'],ssyms++[m'.ssSym]) ((q0,[]),[],ssyms0++[m'.ssSym])` 
+      (`(ID m')^* ((q,[]),[h'],ssyms++[m'.ssSym]) ((q0,[]),[],ssyms0++[m'.ssSym])`
        by METIS_TAC [idcStackInsert] THEN
        `q0 ∈ states m` by METIS_TAC [memStates] THEN
-       `(ID m')^* ((q0,[]),t,ssyms0 ++ [m'.ssSym])	
+       `(ID m')^* ((q0,[]),t,ssyms0 ++ [m'.ssSym])
        ((p,[]),[],ssyms' ++ [m'.ssSym])` by METIS_TAC [stkSymsPdaInv] THEN
        METIS_TAC [idcInpInsert, RTC_RTC, APPEND,APPEND_NIL]) THEN
       `(LENGTH dl' = 0) ∨ (LENGTH dl' = 1)` by DECIDE_TAC THEN1
@@ -750,14 +748,14 @@ THENL[
       SRW_TAC [][] THEN
       `FLAT (MAP h t) = []` by SRW_TAC [][] THEN
       FULL_SIMP_TAC (srw_ss()) [] THEN SRW_TAC [][] THEN
-      `∀e.MEM e t ⇒ (h e = [])` 
+      `∀e.MEM e t ⇒ (h e = [])`
       by (SRW_TAC [][] THEN
 	  FULL_SIMP_TAC (srw_ss()) [rgr_r9eq] THEN
 	  SRW_TAC [][] THEN
 	  FULL_SIMP_TAC (srw_ss()) [MEM_FLAT, MAP_APPEND, FLAT_APPEND]) THEN
       `p ∈ states m` by METIS_TAC [memStates] THEN
 
-      `∃l.ID m' ⊢ l ◁ ((q,[]),[h'],ssyms++[m'.ssSym]) → 
+      `∃l.ID m' ⊢ l ◁ ((q,[]),[h'],ssyms++[m'.ssSym]) →
       ((p,[]),[],ssyms'++[m'.ssSym])`
       by METIS_TAC [rtc2list_exists',idcStackInsert] THEN
       `LENGTH l'' > 1` by (Cases_on `l''`  THEN
@@ -768,21 +766,21 @@ THENL[
       `hInvpda m m' h` by FULL_SIMP_TAC (srw_ss()) [hInvpda,rule1,rule2,
 							   rule3,EXTENSION] THEN
       `stkSymsInPda m' ssyms'` by METIS_TAC [stkSymsPdaInv,NOT_CONS_NIL] THEN
-      `IDC m' ((p,[]),t,ssyms'++[m'.ssSym]) ((p,[]),[],ssyms'++[m'.ssSym])` 
+      `IDC m' ((p,[]),t,ssyms'++[m'.ssSym]) ((p,[]),[],ssyms'++[m'.ssSym])`
       by METIS_TAC [mImpm'HNil,MEM,MEM_APPEND] THEN
       METIS_TAC [APPEND,  RTC_RTC, idcInpInsert,ldImprtc2list,
 		 idcStackInsert],
-      
+
       `(LENGTH l' = 0) ∨ (LENGTH l' = 1)` by DECIDE_TAC THEN1
-      (`l'=[]` by METIS_TAC [LENGTH_NIL] THEN 
+      (`l'=[]` by METIS_TAC [LENGTH_NIL] THEN
        FULL_SIMP_TAC (srw_ss()) [listderiv_def]) THEN
-      
+
       Cases_on `l'` THEN FULL_SIMP_TAC (srw_ss()) [] THEN
       `t'=[]` by METIS_TAC [LENGTH_NIL] THEN
       SRW_TAC [][] THEN
       FULL_SIMP_TAC (srw_ss()) [listderiv_def] THEN
       SRW_TAC [][] THEN
-      `(ID m')^* ((q,[]),t,ssyms++[m'.ssSym]) ((p,[]),[],ssyms'++[m'.ssSym])` 
+      `(ID m')^* ((q,[]),t,ssyms++[m'.ssSym]) ((p,[]),[],ssyms'++[m'.ssSym])`
       by METIS_TAC [APPEND_NIL] THEN
       FULL_SIMP_TAC (srw_ss()) [] THEN
       `h h' = []` by METIS_TAC [] THEN
@@ -792,36 +790,36 @@ THENL[
       SRW_TAC [][] THEN
       IMP_RES_TAC idcStkNil' THEN
       FULL_SIMP_TAC (srw_ss()) [] THEN
-      SRW_TAC [][] 
+      SRW_TAC [][]
       THENL[
 	    Cases_on `dl` THEN FULL_SIMP_TAC (srw_ss()) [] THEN
 	    SRW_TAC [][] THEN
 	    Cases_on `t'` THEN FULL_SIMP_TAC (srw_ss()) [] THEN
 	    Cases_on `h''` THEN Cases_on `r` THEN
-	    FULL_SIMP_TAC (srw_ss()) [id_thm],	    
-	    
+	    FULL_SIMP_TAC (srw_ss()) [id_thm],
+
 	    SRW_TAC [][Once RTC_CASES1] THEN
 	    Q.EXISTS_TAC `((q,[]),t,h''::(t'++[m'.ssSym]))` THEN
 	    FULL_SIMP_TAC (srw_ss()) [rule3, hInvpda, EXTENSION] THEN
 	    `q ∈ states m` by METIS_TAC [memStates,listderiv_def] THEN
-	    `hInvpda m m' h` by FULL_SIMP_TAC (srw_ss()) 
+	    `hInvpda m m' h` by FULL_SIMP_TAC (srw_ss())
 	    [hInvpda,rule1,rule2,rule3,EXTENSION] THEN
 	    `ID m ⊢ dl ◁
 	    (q,FLAT (MAP h t),h''::t') → (p,[],ssyms')`
-	    by FULL_SIMP_TAC (srw_ss()) [listderiv_def] THEN	    
+	    by FULL_SIMP_TAC (srw_ss()) [listderiv_def] THEN
 	    `stkSymsInPda m' (h''::(t' ++ [m'.ssSym]))`
 	    by (FULL_SIMP_TAC (srw_ss()) [] THEN
 		FULL_SIMP_TAC (srw_ss()) [stkSymsInPda] THEN
 		SRW_TAC [][] THEN1
-		METIS_TAC [] THEN1 	    
+		METIS_TAC [] THEN1
 		METIS_TAC [] THEN
 		SRW_TAC [][stkSyms_def]) THEN
 	    `stkSymsInPda m' (ssyms' ++ [m'.ssSym])` by METIS_TAC [stkSymsPdaInv,
 						   APPEND,APPEND_ASSOC] THEN
-	    `ID m' ((q,[]),h'::t,h''::(t' ++ [m'.ssSym])) 
+	    `ID m' ((q,[]),h'::t,h''::(t' ++ [m'.ssSym]))
 	    ((q,[]),t,h''::(t' ++ [m'.ssSym]))` by SRW_TAC [][id_thm] THEN
 	    FULL_SIMP_TAC (srw_ss()) [hInvpda, rule1, rule2,rule3,EXTENSION] THEN
-	    `hInvpda m m' h` by FULL_SIMP_TAC (srw_ss()) 
+	    `hInvpda m m' h` by FULL_SIMP_TAC (srw_ss())
 	    [hInvpda,rule1,rule2,rule3,EXTENSION] THEN
 	    METIS_TAC [stkSymsm'Impm, MEM]
 	    ]]);
@@ -856,7 +854,7 @@ FULL_SIMP_TAC (srw_ss()) [hInvpda, rule1,rule2,rule3,EXTENSION] THEN
 RES_TAC THEN
 SRW_TAC [][] THEN
 FULL_SIMP_TAC (srw_ss()++ARITH_ss) [] THEN
- (`LENGTH (a::q'') ≤ LENGTH q''` 
+ (`LENGTH (a::q'') ≤ LENGTH q''`
   by METIS_TAC [ldIdcInpLen,rtc2list_exists'] THEN
   FULL_SIMP_TAC (srw_ss()++ARITH_ss) []));
 
@@ -880,16 +878,16 @@ Cases_on `r` THEN
 FULL_SIMP_TAC (srw_ss()) [id_thm] THEN
 SRW_TAC [][] THEN
 FULL_SIMP_TAC (srw_ss()) [stkSymsInPda] THEN
-SRW_TAC [][] 
+SRW_TAC [][]
 THENL[
-      Cases_on `pf` THEN FULL_SIMP_TAC (srw_ss()) [] 
+      Cases_on `pf` THEN FULL_SIMP_TAC (srw_ss()) []
       THENL[
 	    SRW_TAC [][] THEN
 	    FULL_SIMP_TAC (srw_ss())  [] THEN
 	    FULL_SIMP_TAC (srw_ss()) [hInvpda,rule1,rule2,rule3,EXTENSION] THEN
 	    SRW_TAC [][] THEN
 	    RES_TAC THEN FULL_SIMP_TAC (srw_ss()) [] THEN
-	    SRW_TAC [][] THEN1	    
+	    SRW_TAC [][] THEN1
 	    METIS_TAC [MEM,memStkSyms,MEM_APPEND,APPEND_11] THEN1
 	    METIS_TAC [MEM,memStkSyms,MEM_APPEND,APPEND_11] THEN1
 	    METIS_TAC [MEM,memStkSyms,MEM_APPEND,APPEND_11] THEN
@@ -918,7 +916,7 @@ THENL[
 		  FULL_SIMP_TAC (srw_ss()) []
 		  ]],
 
-      Cases_on `pf` THEN FULL_SIMP_TAC (srw_ss()) [] 
+      Cases_on `pf` THEN FULL_SIMP_TAC (srw_ss()) []
       THENL[
 	    SRW_TAC [][] THEN
 	    FULL_SIMP_TAC (srw_ss())  [] THEN
@@ -928,8 +926,8 @@ THENL[
 	    `s'=[]` by METIS_TAC [APPEND_11,APPEND_NIL] THEN
 	    SRW_TAC [][] THEN
 	    FULL_SIMP_TAC (srw_ss()) [],
-	    
-	    
+
+
 	    SRW_TAC [][] THEN
 	    `s'=st'++t` by METIS_TAC [APPEND_11,APPEND_ASSOC] THEN
 	    SRW_TAC [][] THEN
@@ -947,9 +945,9 @@ THENL[
 
 val m'ImpmNil = store_thm
 ("m'ImpmNil",
-``∀dl q pfx.ID m' ⊢ dl ◁ ((q,[]),[],pfx++[m'.ssSym]) → 
+``∀dl q pfx.ID m' ⊢ dl ◁ ((q,[]),[],pfx++[m'.ssSym]) →
  ((p,[]),[],ssyms'++[m'.ssSym]) ∧ (q ∈ states m) ∧
- hInvpda m m' h ∧ stkSymsInPda m pfx 
+ hInvpda m m' h ∧ stkSymsInPda m pfx
  ⇒
 IDC m (q,[],pfx) (p,[],ssyms')``,
 
@@ -975,11 +973,11 @@ THENL[
       METIS_TAC [memStkSyms] THEN
       `(q0,[]) = (q,[])` by METIS_TAC [] THEN
       FULL_SIMP_TAC (srw_ss()) [] THEN SRW_TAC [][],
-      
+
       FULL_SIMP_TAC (srw_ss()) [] THEN
       FULL_SIMP_TAC (srw_ss()) [hInvpda,rule1,rule2,rule3,EXTENSION] THEN
       RES_TAC THEN FULL_SIMP_TAC (srw_ss()) [] THEN SRW_TAC [][] THEN
-      `hInvpda m m' h` by FULL_SIMP_TAC (srw_ss()) 
+      `hInvpda m m' h` by FULL_SIMP_TAC (srw_ss())
       [hInvpda,rule1,rule2,rule3,EXTENSION] THENL[
       `stkSymsInPda m ssyms` by METIS_TAC [memStkSyms, stkSymsInPda] THEN
       `stkSymsInPda m ssyms` by METIS_TAC [stkSymsInPda,memStkSyms] THEN
@@ -999,7 +997,7 @@ val m'StepBufToNil = store_thm
 ("m'StepBufToNil",
 ``∀dl q b x pfx.
 ID m' ⊢ dl ◁ ((q,b),x,pfx++[m'.ssSym]) → ((p,[]),[],ssyms'++[m'.ssSym]) ∧
-hInvpda m m' h 
+hInvpda m m' h
 ⇒
 ∃q0 ssyms0.
 IDC m' ((q,b),x,pfx++[m'.ssSym]) ((q0,[]),x,ssyms0++[m'.ssSym]) ∧
@@ -1023,7 +1021,7 @@ SRW_TAC [][]
 THENL[
       Cases_on `pfx` THEN FULL_SIMP_TAC (srw_ss()) [] THEN
       SRW_TAC [][] THEN FULL_SIMP_TAC (srw_ss()) [] THEN
-      RES_TAC THEN FULL_SIMP_TAC (srw_ss()) [] THEN SRW_TAC [][] 
+      RES_TAC THEN FULL_SIMP_TAC (srw_ss()) [] THEN SRW_TAC [][]
       THENL[
 	    METIS_TAC [memStkSyms],
 	    METIS_TAC [memStkSyms],
@@ -1038,10 +1036,10 @@ THENL[
 	    FULL_SIMP_TAC (srw_ss()) [] THEN
 	    METIS_TAC [RTC_RULES,RTC_RTC],
 
-	    
+
 	    FIRST_X_ASSUM (Q.SPECL_THEN [`p'`,`b`,`q'`,`ssyms++t'`] MP_TAC) THEN
 	    SRW_TAC [][] THEN
-	    `ID m' ((q,b),q',h'::(t' ++ [m'.ssSym])) 
+	    `ID m' ((q,b),q',h'::(t' ++ [m'.ssSym]))
 	    ((p',b),q',ssyms ++ t' ++ [m'.ssSym])`
 	    by (SRW_TAC [][id_thm] THEN METIS_TAC []) THEN
 	    Q.EXISTS_TAC `q0''` THEN Q.EXISTS_TAC `ssyms0'`THEN
@@ -1049,7 +1047,7 @@ THENL[
 	    METIS_TAC [RTC_RULES,RTC_RTC],
 
 
-	    `ID m' ((q,isym::r'),q',h'::(t' ++ [m'.ssSym])) 
+	    `ID m' ((q,isym::r'),q',h'::(t' ++ [m'.ssSym]))
 	    ((p',r'),q',ssyms ++ t' ++ [m'.ssSym])`
 	    by (SRW_TAC [][id_thm] THEN
 		METIS_TAC []) THEN
@@ -1060,7 +1058,7 @@ THENL[
 	    `(q,b) = (q0,[])` by METIS_TAC [] THEN
 	    FULL_SIMP_TAC (srw_ss()) [] THEN SRW_TAC [][] THEN
 	    RES_TAC THEN FULL_SIMP_TAC (srw_ss()) [] THEN SRW_TAC [][] THEN
-	    `ID m'  (m'.start,q',m'.ssSym::t'++[m'.ssSym]) 
+	    `ID m'  (m'.start,q',m'.ssSym::t'++[m'.ssSym])
 	     ((m.start,[]),q',m.ssSym::m'.ssSym::(t' ++ [m'.ssSym]))`
 	    by (SRW_TAC [][id_thm] THEN
 		METIS_TAC [APPEND,APPEND_ASSOC]) THEN
@@ -1071,7 +1069,7 @@ THENL[
 
       Cases_on `pfx` THEN FULL_SIMP_TAC (srw_ss()) [] THEN
       SRW_TAC [][] THEN FULL_SIMP_TAC (srw_ss()) [] THEN
-      RES_TAC THEN FULL_SIMP_TAC (srw_ss()) [] THEN SRW_TAC [][] 
+      RES_TAC THEN FULL_SIMP_TAC (srw_ss()) [] THEN SRW_TAC [][]
       THENL[
 	    FIRST_X_ASSUM (Q.SPECL_THEN [`q`,`h a`,`q'`,`[]`] MP_TAC) THEN
 	    SRW_TAC [][] THEN
@@ -1082,7 +1080,7 @@ THENL[
 	    SRW_TAC [][] THEN
 	    METIS_TAC [RTC_RULES,RTC_RTC],
 
-	    
+
 	    FIRST_X_ASSUM (Q.SPECL_THEN [`q`,`h a`,`q'`,`h'::t'`] MP_TAC) THEN
 	    SRW_TAC [][] THEN
 	    `ID m' ((q,[]),a::q',h'::(t' ++ [m'.ssSym]))
@@ -1112,7 +1110,7 @@ val m'StepBufNilH = store_thm
 ("m'StepBufNilH",
 ``∀dl p b ssyms'.
 ID m' ⊢ dl ◁ ((q,[]),[e],pfx++[m'.ssSym]) → ((p,b),[],ssyms'++[m'.ssSym]) ∧
-hInvpda m m' h 
+hInvpda m m' h
 ⇒
 ∃q0 ssyms0.
 IDC m' ((q,[]),[e],pfx++[m'.ssSym]) ((q0,h e),[],ssyms0++[m'.ssSym]) ∧
@@ -1134,14 +1132,14 @@ FULL_SIMP_TAC (srw_ss()) [id_thm] THEN SRW_TAC [][] THEN
 FULL_SIMP_TAC (srw_ss()) [hInvpda,rule1,rule2,rule3,EXTENSION] THEN
 SRW_TAC [][]
  THENL[
-       `hInvpda m m' h` by 
+       `hInvpda m m' h` by
        FULL_SIMP_TAC (srw_ss()) [rule1,rule2,rule3,hInvpda, EXTENSION] THEN
        `MEM ((q'',r'),[],sh::st) dl` by METIS_TAC [MEM,MEM_APPEND] THEN
        `∃pf.sh::st = pf ++[m'.ssSym]` by METIS_TAC [z0Inv,memld] THEN
        SRW_TAC [][] THEN
        Cases_on `pf` THEN FULL_SIMP_TAC (srw_ss()) [] THEN
        SRW_TAC [][] THEN FULL_SIMP_TAC (srw_ss()) [] THEN
-       RES_TAC THEN FULL_SIMP_TAC (srw_ss()) [] THEN SRW_TAC [][] 
+       RES_TAC THEN FULL_SIMP_TAC (srw_ss()) [] THEN SRW_TAC [][]
        THENL[
 	     METIS_TAC [memStkSyms],
 	     METIS_TAC [memStkSyms],
@@ -1182,7 +1180,7 @@ SRW_TAC [][]
 	     FIRST_X_ASSUM (Q.SPECL_THEN [`q''`,`[]`,`m'.ssSym::t`] MP_TAC) THEN
 	    SRW_TAC [][] THEN
 	    `ID m' (m'.start,[],m'.ssSym::(t ++ [m'.ssSym]))
-	     ((m.start,[]),[],m.ssSym::m'.ssSym::(t ++ [m'.ssSym]))`	    
+	     ((m.start,[]),[],m.ssSym::m'.ssSym::(t ++ [m'.ssSym]))`
 	    by (SRW_TAC [][id_thm] THEN
 		METIS_TAC [APPEND,APPEND_ASSOC]) THEN
 	    Q.EXISTS_TAC `q0` THEN Q.EXISTS_TAC `ssyms0`THEN
@@ -1190,13 +1188,13 @@ SRW_TAC [][]
 	    METIS_TAC [RTC_RULES_RIGHT1,RTC_RTC]
 	    ],
 
-       `hInvpda m m' h` by 
+       `hInvpda m m' h` by
        FULL_SIMP_TAC (srw_ss()) [rule1,rule2,rule3,hInvpda, EXTENSION] THEN
        `∃pf.sh::st = pf ++[m'.ssSym]` by METIS_TAC [z0Inv,memld] THEN
        SRW_TAC [][] THEN
        Cases_on `pf` THEN FULL_SIMP_TAC (srw_ss()) [] THEN
        SRW_TAC [][] THEN FULL_SIMP_TAC (srw_ss()) [] THEN
-       RES_TAC THEN FULL_SIMP_TAC (srw_ss()) [] THEN SRW_TAC [][] 
+       RES_TAC THEN FULL_SIMP_TAC (srw_ss()) [] THEN SRW_TAC [][]
       THENL[
 	    `ssyms'=[]` by METIS_TAC [APPEND_NIL,APPEND_11] THEN
 	    SRW_TAC [][] THEN
@@ -1213,7 +1211,7 @@ SRW_TAC [][]
 	    SRW_TAC [][] THEN
 	    METIS_TAC [RTC_RULES_RIGHT1,RTC_RTC,ldImprtc2list],
 
-	    `ID m' ((p,[]),[a],h'::(t ++ [m'.ssSym])) 
+	    `ID m' ((p,[]),[a],h'::(t ++ [m'.ssSym]))
 	    ((p,h a),[],h'::(t ++ [m'.ssSym]))`
 	    by SRW_TAC [][id_thm] THEN
 	    IMP_RES_TAC ldIdcInpSuffix THEN
@@ -1226,7 +1224,7 @@ SRW_TAC [][]
 	    SRW_TAC [][] THEN
 	    METIS_TAC [RTC_RULES_RIGHT1,RTC_RTC,ldImprtc2list],
 
-	    `ID m' ((p,[]),[a],m'.ssSym::(t ++ [m'.ssSym])) 
+	    `ID m' ((p,[]),[a],m'.ssSym::(t ++ [m'.ssSym]))
 	    ((p,h a),[],m'.ssSym::(t ++ [m'.ssSym]))`
 	    by SRW_TAC [][id_thm] THEN
 	    IMP_RES_TAC ldIdcInpSuffix THEN
@@ -1237,7 +1235,7 @@ SRW_TAC [][]
 	    Q.EXISTS_TAC `p` THEN
 	    Q.EXISTS_TAC `m'.ssSym::t` THEN
 	    SRW_TAC [][] THEN
-	    METIS_TAC [RTC_RULES_RIGHT1,RTC_RTC,ldImprtc2list]	    
+	    METIS_TAC [RTC_RULES_RIGHT1,RTC_RTC,ldImprtc2list]
 	    ]]);
 
 
@@ -1268,7 +1266,7 @@ SRW_TAC [][]
 THENL[
       Cases_on `pfx` THEN FULL_SIMP_TAC (srw_ss()) [] THEN
       SRW_TAC [][] THEN FULL_SIMP_TAC (srw_ss()) [] THEN
-      RES_TAC THEN FULL_SIMP_TAC (srw_ss()) [] THEN SRW_TAC [][] 
+      RES_TAC THEN FULL_SIMP_TAC (srw_ss()) [] THEN SRW_TAC [][]
       THENL[
 	    METIS_TAC [memStkSyms],
 	    METIS_TAC [memStkSyms],
@@ -1278,7 +1276,7 @@ THENL[
 	    FIRST_X_ASSUM (Q.SPECL_THEN [`m.start`,`[]`,`q'`,`[m.ssSym]`] MP_TAC) THEN
 	    SRW_TAC [][] THEN
 	    `ID m (q,b,h'::t') (p',b,ssyms ++ t')` by SRW_TAC [][id_thm] THEN
-	    METIS_TAC [RTC_RULES],	    
+	    METIS_TAC [RTC_RULES],
 
 	    `p' ∈ states m` by (SRW_TAC [][states_def, EXTENSION] THEN
 				METIS_TAC []) THEN
@@ -1316,10 +1314,10 @@ val m'isSuff = store_thm
 ("m'isSuff",
 ``∀dl q' b ssyms'.
 ID m' ⊢ dl ◁ ((q,[]),[h'],pfx ++ [m'.ssSym]) → ((q',b),[],ssyms' ++ [m'.ssSym]) ∧
-hInvpda m m' h 
+hInvpda m m' h
 ⇒
 isSuffix b (h h')``,
-	     
+
 HO_MATCH_MP_TAC SNOC_INDUCT THEN SRW_TAC [] [SNOC_APPEND]  THEN1
 FULL_SIMP_TAC (srw_ss()) [listderiv_def] THEN
 Cases_on `dl=[]` THEN FULL_SIMP_TAC (srw_ss()) [] THEN1
@@ -1342,7 +1340,7 @@ SRW_TAC [][]
        SRW_TAC [][] THEN
        Cases_on `pf` THEN FULL_SIMP_TAC (srw_ss()) [] THEN
        SRW_TAC [][] THEN FULL_SIMP_TAC (srw_ss()) [] THEN
-       RES_TAC THEN FULL_SIMP_TAC (srw_ss()) [] THEN SRW_TAC [][] 
+       RES_TAC THEN FULL_SIMP_TAC (srw_ss()) [] THEN SRW_TAC [][]
        THENL[
 	     METIS_TAC [memStkSyms],
 	     METIS_TAC [memStkSyms],
@@ -1375,7 +1373,7 @@ SRW_TAC [][]
        SRW_TAC [][] THEN
        Cases_on `pf` THEN FULL_SIMP_TAC (srw_ss()) [] THEN
        SRW_TAC [][] THEN FULL_SIMP_TAC (srw_ss()) [] THEN
-       RES_TAC THEN FULL_SIMP_TAC (srw_ss()) [] THEN SRW_TAC [][] 
+       RES_TAC THEN FULL_SIMP_TAC (srw_ss()) [] THEN SRW_TAC [][]
        THEN1
 	     (`ssyms'=[]` by METIS_TAC [APPEND_11,APPEND_NIL] THEN
 	     SRW_TAC [][] THEN FULL_SIMP_TAC (srw_ss()) [] THEN
@@ -1396,7 +1394,7 @@ SRW_TAC [][]
 	     SRW_TAC [][] THEN
 	     FULL_SIMP_TAC (srw_ss()) [] THEN
 	     METIS_TAC [IS_PREFIX_APPEND, APPEND_NIL])]);
-	     
+
 
 val m'ImpmhTohh' = store_thm
 ("m'ImpmhTohh'",
@@ -1421,7 +1419,7 @@ Cases_on `r` THEN
 FULL_SIMP_TAC (srw_ss()) [id_thm] THEN SRW_TAC [][] THEN
 FULL_SIMP_TAC (srw_ss()) [hInvpda,rule1,rule2,rule3,EXTENSION] THEN
 SRW_TAC [][] THEN
- `hInvpda m m' h ` by 
+ `hInvpda m m' h ` by
  FULL_SIMP_TAC (srw_ss()) [hInvpda,rule1,rule2,
 			   rule3,EXTENSION]
  THENL[
@@ -1431,7 +1429,7 @@ SRW_TAC [][] THEN
        SRW_TAC [][] THEN
        Cases_on `pf` THEN FULL_SIMP_TAC (srw_ss()) [] THEN
        SRW_TAC [][] THEN FULL_SIMP_TAC (srw_ss()) [] THEN
-       RES_TAC THEN FULL_SIMP_TAC (srw_ss()) [] THEN SRW_TAC [][] 
+       RES_TAC THEN FULL_SIMP_TAC (srw_ss()) [] THEN SRW_TAC [][]
        THENL[
 	     METIS_TAC [memStkSyms],
 	     METIS_TAC [memStkSyms],
@@ -1451,7 +1449,7 @@ SRW_TAC [][] THEN
 	     `t=[]` by METIS_TAC [LENGTH_NIL] THEN
 	     SRW_TAC [][] THEN
 	     FULL_SIMP_TAC (srw_ss()) [],
-	    
+
 
 	     FIRST_X_ASSUM (Q.SPECL_THEN [`q''`,`h''::t`] MP_TAC) THEN
 	     SRW_TAC [][] THEN
@@ -1468,7 +1466,7 @@ SRW_TAC [][] THEN
 
 	     `(q''',r') = (q0,[])` by METIS_TAC [] THEN
 	     FULL_SIMP_TAC (srw_ss()) [] THEN SRW_TAC [][] THEN
-	     `IDC m (q,[],pfx) (q''',[],m'.ssSym::t)` 
+	     `IDC m (q,[],pfx) (q''',[],m'.ssSym::t)`
 	     by METIS_TAC [APPEND,APPEND_NIL] THEN
 	     `∃dl.ID m ⊢ dl ◁ (q,[],pfx) → (q''',[],m'.ssSym::t)`
 	     by METIS_TAC [ rtc2list_exists'] THEN
@@ -1488,7 +1486,7 @@ SRW_TAC [][] THEN
        SRW_TAC [][] THEN
        Cases_on `pf` THEN FULL_SIMP_TAC (srw_ss()) [] THEN
        SRW_TAC [][] THEN FULL_SIMP_TAC (srw_ss()) [] THEN
-       RES_TAC THEN FULL_SIMP_TAC (srw_ss()) [] THEN SRW_TAC [][] 
+       RES_TAC THEN FULL_SIMP_TAC (srw_ss()) [] THEN SRW_TAC [][]
        THENL[
 	     IMP_RES_TAC ldIdcInpSuffix THEN
 	    FULL_SIMP_TAC (srw_ss()) [] THEN SRW_TAC [][] THEN
@@ -1551,10 +1549,10 @@ FULL_SIMP_TAC (srw_ss()) [id_thm] THEN SRW_TAC [][] THEN
 
 val m'Impm = store_thm
 ("m'Impm",
-``∀dl q pfx. 
- ID m' ⊢ dl ◁ ((q,[]),x,pfx++[m'.ssSym]) → ((p,[]),[],ssyms'++[m'.ssSym]) ∧ 
+``∀dl q pfx.
+ ID m' ⊢ dl ◁ ((q,[]),x,pfx++[m'.ssSym]) → ((p,[]),[],ssyms'++[m'.ssSym]) ∧
 stkSymsInPda m pfx ∧ q ∈ states m ∧
- hInvpda (m:(α, β, γ) pda) (m':(α, β, γ # α list) pda) (h: α -> α list) 
+ hInvpda (m:(α, β, γ) pda) (m':(α, β, γ # α list) pda) (h: α -> α list)
  ⇒
  ∃dl'.ID m ⊢ dl' ◁ (q,FLAT (MAP h x),pfx) → (p,[],ssyms')``,
 
@@ -1562,7 +1560,7 @@ Induct_on `x` THEN
 SRW_TAC [][] THEN1
 (IMP_RES_TAC m'ImpmNil THEN
  METIS_TAC [rtc2list_exists']) THEN
-`ID m' ⊢ dl ◁ ((q,[]),[h']++x,pfx++[m'.ssSym]) → ((p,[]),[],ssyms'++[m'.ssSym])` 
+`ID m' ⊢ dl ◁ ((q,[]),[h']++x,pfx++[m'.ssSym]) → ((p,[]),[],ssyms'++[m'.ssSym])`
 by METIS_TAC [APPEND] THEN
 IMP_RES_TAC idTransOnInpPfx THEN
  `IDC m' ((q,[]),[h'],pfx++[m'.ssSym]) (q0,[],ssyms0)`
@@ -1572,7 +1570,7 @@ SRW_TAC [][] THEN
  `stkSymsInPda m p'` by METIS_TAC [stkSymsPdaInvm'm] THEN
 Cases_on `q0` THEN
 `∃q0 ssyms0.IDC m' ((q',r),x,p' ++ [m'.ssSym]) ((q0,[]),x,ssyms0 ++ [m'.ssSym]) ∧
-IDC m' ((q0,[]),x,ssyms0 ++ [m'.ssSym]) ((p,[]),[],ssyms' ++ [m'.ssSym])` 
+IDC m' ((q0,[]),x,ssyms0 ++ [m'.ssSym]) ((p,[]),[],ssyms' ++ [m'.ssSym])`
 by METIS_TAC [m'StepBufToNil, rtc2list_exists',ldImprtc2list] THEN
 `stkSymsInPda m ssyms0` by METIS_TAC [stkSymsPdaInvm'm, RTC_RTC] THEN
 `q0 ∈ states m` by METIS_TAC [ RTC_RTC, rtc2list_exists',m'StateImpm] THEN
@@ -1580,11 +1578,11 @@ by METIS_TAC [m'StepBufToNil, rtc2list_exists',ldImprtc2list] THEN
  by METIS_TAC [rtc2list_exists'] THEN
 SRW_TAC [][] THEN
 `q' ∈ states m` by METIS_TAC [ RTC_RTC, rtc2list_exists',m'StateImpm] THEN
-`IDC m (q',r,p') (q0,[],ssyms0)` by METIS_TAC [m'ImpmBufInpSame, 
+`IDC m (q',r,p') (q0,[],ssyms0)` by METIS_TAC [m'ImpmBufInpSame,
 					       rtc2list_exists'] THEN
-`∃q0 ssyms0.IDC m' ((q,[]),[h'],pfx ++ [m'.ssSym]) 
+`∃q0 ssyms0.IDC m' ((q,[]),[h'],pfx ++ [m'.ssSym])
 ((q0,h h'),[],ssyms0 ++ [m'.ssSym]) ∧
-IDC m' ((q0,h h'),[],ssyms0 ++ [m'.ssSym]) ((q',r),[],p' ++ [m'.ssSym])` 
+IDC m' ((q0,h h'),[],ssyms0 ++ [m'.ssSym]) ((q',r),[],p' ++ [m'.ssSym])`
 by METIS_TAC [m'StepBufNilH,rtc2list_exists'] THEN
 `q0' ∈ states m` by METIS_TAC [ RTC_RTC, rtc2list_exists',m'StateImpm] THEN
 `IDC m (q0',h h',ssyms0') (q',r,p')` by METIS_TAC [m'ImpmBufInpSame,
@@ -1595,7 +1593,7 @@ IMP_RES_TAC ldImprtc2list THEN
 by METIS_TAC [RTC_RTC] THEN
 `(ID m)^* (q0',h h'++ FLAT (MAP h x),ssyms0') (q0,FLAT (MAP h x),ssyms0)`
 by METIS_TAC [idcInpInsert, APPEND_NIL] THEN
-`IDC m (q,[],pfx) (q0',[],ssyms0')` by 
+`IDC m (q,[],pfx) (q0',[],ssyms0')` by
 METIS_TAC [m'ImpmhTohh',hInvpda,rtc2list_exists'] THEN
 METIS_TAC [RTC_RTC,rtc2list_exists',idcInpInsert,APPEND_NIL]);
 
@@ -1604,7 +1602,7 @@ METIS_TAC [RTC_RTC,rtc2list_exists',idcInpInsert,APPEND_NIL]);
 val m'FstStep = store_thm
 ("m'FstStep",
 ``ID m' ⊢ l ◁ (m'.start,x,[m'.ssSym]) → (state,[],stack) ∧
-(state ≠ m'.start) ∧ hInvpda m m' h 
+(state ≠ m'.start) ∧ hInvpda m m' h
 ⇒
 ID m' ⊢ TL l ◁ ((m.start,[]),x,[m.ssSym]++[m'.ssSym]) → (state,[],stack)``,
 
@@ -1642,10 +1640,10 @@ SRW_TAC [][stkSymsInPda] THEN
 METIS_TAC [memStkSymsEq,MEM]);
 
 
-val invhEq = store_thm 
+val invhEq = store_thm
 ("invhEq",
 ``∀m m'. hInvpda m m' h
- ⇒ 
+ ⇒
  (x ∈ lafs m' = x ∈ { w | (FLAT (MAP h w)) ∈ lafs m })``,
 
 SRW_TAC [][EXTENSION, language_def, EQ_IMP_THM, lafs_def] THEN
@@ -1694,8 +1692,8 @@ THENL[
 				       FULL_SIMP_TAC (srw_ss()) [FLAT_APPEND]) THEN
       `m.start ∈ states m` by SRW_TAC [][states_def] THEN
       `stkSymsInPda m' [m.ssSym]` by METIS_TAC [mSsymInm'] THEN
-      `IDC m' ((m.start,[]),x,[m.ssSym] ++ [m'.ssSym]) 
-              ((m.start,[]),[],[m.ssSym] ++ [m'.ssSym])` 
+      `IDC m' ((m.start,[]),x,[m.ssSym] ++ [m'.ssSym])
+              ((m.start,[]),[],[m.ssSym] ++ [m'.ssSym])`
       by METIS_TAC [mImpm'HNil] THEN
       SRW_TAC [][Once RTC_CASES1] THEN
       Q.EXISTS_TAC `(m.start,[])` THEN
@@ -1708,33 +1706,244 @@ THENL[
       FULL_SIMP_TAC (srw_ss()) [hInvpda]
       ]);
 
-val inverseHomomorphism = Define 
+
+val inverseHomomorphism = Define
 `inverseHomomorphism h (g:('nts,'ts)grammar) = { w | (FLAT (MAP h w)) ∈ language g}`;
- 
 
-``∀g (h:('nts, 'ts) symbol -> ('nts, 'ts) symbol list). INFINITE
-(UNIV:'nts set) ∧ [] ∉ language (g:('nts,'ts) grammar) ⇒ ∃g'. language
-g' = inverseHomomorphism h g``
+val GSPEC_IMAGE = store_thm(
+  "GSPEC_IMAGE",
+  ``GSPEC f = IMAGE (FST o f) { x | SND (f x) }``,
+  SRW_TAC [][EXTENSION, GSPECIFICATION, SPECIFICATION] THEN
+  EQ_TAC THEN SRW_TAC [][] THEN Q.EXISTS_TAC `x'` THEN SRW_TAC [][] THEN
+  Cases_on `f x'` THEN FULL_SIMP_TAC (srw_ss()) []);
 
-SRW_TAC [][]
-`∃g'.isGnf g' ∧ (language g = language g')` by METIS_TAC [gnfExists]
+val f2GSPEC = prove(
+  ``(\x. p x) = GSPEC (S $, p)``,
+  SRW_TAC [][EXTENSION, GSPECIFICATION] THEN SRW_TAC [][SPECIFICATION])
 
+val uc2GSPEC = prove(
+  ``UNCURRY (\a b. p a b) = GSPEC (UNCURRY (S (S o ($o $,) o $,) p))``,
+  SIMP_TAC (srw_ss()) [EXTENSION, GSPECIFICATION, pairTheory.EXISTS_PROD,
+                       pairTheory.FORALL_PROD] THEN
+  SRW_TAC [][SPECIFICATION]);
+
+open boolSimps
+val lemma =
+  SIMP_RULE (srw_ss()) [] (Q.INST [`P` |-> `λl0. h::l = l0 ++ m`]
+                                  EXISTS_LIST)
+val suffixes_are_finite = store_thm(
+  "suffixes_are_finite",
+  ``∀l. FINITE { m | isSuffix m l }``,
+  SIMP_TAC (srw_ss()) [isSuffix_APPEND] THEN
+  Induct_on `l` THEN SRW_TAC [][lemma, GSPEC_OR]);
+
+val FINITE_isSuffixTrans = store_thm(
+  "FINITE_isSuffixTrans",
+  ``FINITE univ(:'a) ⇒
+    FINITE {((opt,q,r,x),(q',x),r') | (x,a:'a) | isSuffix x (h a)}``,
+  STRIP_TAC THEN ONCE_REWRITE_TAC [GSPEC_IMAGE] THEN
+  MATCH_MP_TAC IMAGE_FINITE THEN
+  SRW_TAC [][PAIR_ABS] THEN
+  MATCH_MP_TAC SUBSET_FINITE_I THEN
+  Q.EXISTS_TAC `(BIGUNION (IMAGE (\a. { l | isSuffix l (h a)}) univ(:'a)))
+                   CROSS
+                univ(:'a)` THEN
+  Tactical.REVERSE (SRW_TAC [DNF_ss][SUBSET_DEF]) THEN1 METIS_TAC [] THEN
+  SRW_TAC [][suffixes_are_finite]);
+
+val GSPEC' = REWRITE_RULE [SPECIFICATION] GSPECIFICATION
+
+val GSPEC_AND = prove(
+  ``{ x | p x /\ q x } = {x | p x} ∩ {x | q x}``,
+  SRW_TAC [][EXTENSION])
+
+val uc1_gs = prove(
+  ``UNCURRY (\x. GSPEC (f x)) =
+    GSPEC (UNCURRY (S (S o ($o $,) o $,) (combin$C $IN o GSPEC o f)))``,
+  SIMP_TAC (srw_ss()) [EXTENSION, pairTheory.FORALL_PROD, GSPECIFICATION,
+                       pairTheory.EXISTS_PROD] THEN
+  SRW_TAC [][SPECIFICATION, GSPEC'])
+
+val PAIR_ABS = prove(
+  ``(\x. f x) = (λ(a,b). f (a,b))``,
+  SIMP_TAC (srw_ss())[FUN_EQ_THM, pairTheory.FORALL_PROD]);
+
+val UNCURRY' = prove(
+  ``UNCURRY f = \v. f (FST v) (SND v)``,
+  SIMP_TAC (srw_ss()) [pairTheory.FORALL_PROD,FUN_EQ_THM]
+  )
+
+val FINITE_INTER2 = store_thm(
+  "FINITE_INTER2",
+  ``FINITE s2 ⇒ FINITE (s1 ∩ s2)``,
+  METIS_TAC [INTER_FINITE, INTER_COMM])
+
+val FINITE_rule1 = store_thm("FINITE_rule1",
+  ``FINITE univ(:'a) ⇒
+    FINITE (rule1 (m:(α, β, γ) pda) (h: α -> α list))``,
+
+SRW_TAC [][rule1] THEN
+Q.MATCH_ABBREV_TAC `FINITE Horrible` THEN
+Q.ABBREV_TAC `
+  (f:(α, β, γ) trans -> (α, β, γ # α list) trans -> bool) =
+   \r. case r of
+         ((NONE,ssym,q),p,ssyms) =>
+           if (∃a x. isSuffix x (h a) ∧ ((NONE,ssym,q),p,ssyms) ∈ m.next)
+           then
+             { ((NONE:α option,ssym,q,x),(p,x),ssyms) | x, a |
+               isSuffix x (h a)
+             }
+           else {}
+       | otherwise => {}
+` THEN
+Q_TAC SUFF_TAC `Horrible = BIGUNION (IMAGE f  (set m.next))` THEN
+ASM_SIMP_TAC (srw_ss()) [] THEN1
+
+(ASM_SIMP_TAC (srw_ss() ++ boolSimps.DNF_ss)
+              [EXISTS_rule, pairTheory.FORALL_PROD, Abbr`f`] THEN
+ Q.X_GEN_TAC `v` THEN Cases_on `v` THEN SRW_TAC [][] THEN
+ METIS_TAC [FINITE_isSuffixTrans]) THEN
+
+ONCE_REWRITE_TAC [EXTENSION] THEN
+ASM_SIMP_TAC (srw_ss() ++ DNF_ss) [Abbr`f`, Abbr`Horrible`] THEN
+ASM_SIMP_TAC (srw_ss() ++ DNF_ss) [pairTheory.FORALL_PROD,
+                                   pairTheory.EXISTS_PROD,
+                                   EXISTS_OPTION] THEN
+SIMP_TAC (srw_ss() ++ COND_elim_ss ++ DNF_ss ++ CONJ_ss) [] THEN
+METIS_TAC []);
+
+val FINITE_rule2 = store_thm(
+  "FINITE_rule2",
+  ``FINITE univ(:'a) ⇒ FINITE (rule2 (m:(α, β, γ) pda) (h: α -> α list))``,
+
+SRW_TAC [][rule2] THEN
+Q.MATCH_ABBREV_TAC `FINITE Horrible` THEN
+Q.ABBREV_TAC `
+  (f:(α, β, γ) trans -> (α, β, γ # α list) trans -> bool) =
+  \r. case r of
+        ((SOME isym,ssym,q),p,ssyms) =>
+           if (∃a x. isSuffix (isym::x) (h a) ∧
+                     ((SOME isym,ssym,q),p,ssyms) ∈ m.next)
+           then
+             { ((NONE:α option,ssym,q,isym::x),(p,x),ssyms) | x, a|
+               isSuffix (isym::x) (h a)
+             }
+           else {}
+      | otherwise => {}
+` THEN
+Q_TAC SUFF_TAC `Horrible = BIGUNION (IMAGE f  (set m.next))` THEN
+ASM_SIMP_TAC (srw_ss()) [] THEN1
+   (ASM_SIMP_TAC (srw_ss() ++ DNF_ss)
+                 [pairTheory.FORALL_PROD, Abbr`f`] THEN
+    ASM_SIMP_TAC (srw_ss()) [FORALL_OPTION] THEN
+    SRW_TAC [][] THEN
+    ONCE_REWRITE_TAC [GSPEC_IMAGE] THEN
+    MATCH_MP_TAC IMAGE_FINITE THEN
+    SRW_TAC [][PAIR_ABS] THEN
+    MATCH_MP_TAC SUBSET_FINITE_I THEN
+    Q.EXISTS_TAC `
+      (BIGUNION (IMAGE (\a. { l | isSuffix (x::l) (h a)}) univ(:'a)))
+                   CROSS
+      univ(:'a)` THEN
+    Tactical.REVERSE (SRW_TAC [DNF_ss][SUBSET_DEF]) THEN1 METIS_TAC [] THEN
+    DISJ2_TAC THEN Q.X_GEN_TAC `v` THEN
+    MATCH_MP_TAC SUBSET_FINITE_I THEN
+    Q.EXISTS_TAC `{l | isSuffix l (h v)}` THEN CONJ_TAC THEN1
+    SRW_TAC [][suffixes_are_finite] THEN
+    SIMP_TAC (srw_ss()) [SUBSET_DEF, isSuffix_APPEND] THEN
+    SRW_TAC [][] THEN SRW_TAC [][] THEN Q.EXISTS_TAC `l0 ++ [x]` THEN
+    METIS_TAC [APPEND, APPEND_ASSOC]) THEN
+
+ONCE_REWRITE_TAC [EXTENSION] THEN
+ASM_SIMP_TAC (srw_ss() ++ DNF_ss) [Abbr`f`, Abbr`Horrible`] THEN
+ASM_SIMP_TAC (srw_ss() ++ DNF_ss) [pairTheory.FORALL_PROD,
+                                   pairTheory.EXISTS_PROD,
+                                   EXISTS_OPTION] THEN
+SIMP_TAC (srw_ss() ++ COND_elim_ss ++ DNF_ss ++ CONJ_ss) [] THEN
+METIS_TAC []);
+
+val FINITE_rule3 = store_thm(
+  "FINITE_rule3",
+  ``FINITE univ(:'a) ⇒
+    FINITE (rule3 (m:(α, β, γ) pda) (h: α -> α list) newssym)``,
+
+  SRW_TAC [][rule3] THEN
+  ONCE_REWRITE_TAC [GSPEC_IMAGE] THEN
+  SRW_TAC [][PAIR_ABS] THEN
+  MATCH_MP_TAC IMAGE_FINITE THEN
+  MATCH_MP_TAC SUBSET_FINITE_I THEN
+  Q.EXISTS_TAC `univ(:'a) × ((newssym INSERT stkSyms m) × states m)`  THEN
+  SRW_TAC [][finiteStkSyms, finiteStates] THEN
+  SRW_TAC [][SUBSET_DEF] THEN SRW_TAC [][]);
+
+val FINITE_finalStateSet = store_thm("FINITE_finalStateSet",
+``FINITE {(q,[]:(α, β) symbol list) | q ∈ m.final}``,
+Q.MATCH_ABBREV_TAC `FINITE Horrible` THEN
+Q.ABBREV_TAC `f = \q. if (q ∈ m.final) then {(q,[]:(α, β) symbol list)} else {}` THEN
+Q_TAC SUFF_TAC `Horrible = BIGUNION (IMAGE f (set m.final))` THEN1
+SRW_TAC [boolSimps.COND_elim_ss, boolSimps.DNF_ss,
+            boolSimps.CONJ_ss][EXISTS_rule,
+                               Abbr`f`] THEN
+ONCE_REWRITE_TAC [EXTENSION] THEN
+SRW_TAC [boolSimps.COND_elim_ss, boolSimps.DNF_ss,
+            boolSimps.CONJ_ss][EXISTS_rule, Abbr`Horrible`, Abbr`f`]);
+
+
+val exists_hInvpda = store_thm ("exists_hInvpda",
+  ``INFINITE univ(:γ) ∧ INFINITE univ(:δ) ∧ FINITE univ(:(α,β)symbol) ⇒
+    ∀(m: ((α, β) symbol, γ, δ) pda) h. ∃m'. hInvpda m m' h``,
+
+  SRW_TAC [][hInvpda] THEN
+  `FINITE (stkSyms m)`
+       by METIS_TAC [finiteStkSyms, FINITE_LIST_TO_SET] THEN
+  `∃x0. x0 ∈ (univ((:γ) :γ itself)) ∧ ~(x0 ∈ (stkSyms m))`
+      by METIS_TAC [IN_INFINITE_NOT_FINITE, new_ssym_exists] THEN
+  `FINITE (set (statesList m))` by SRW_TAC [][] THEN
+  `∃q0. q0 ∉ states m`
+     by METIS_TAC [new_state_exists, states_list_eqresult] THEN
+  `FINITE ((rule1 m h ∪ rule2 m h ∪ rule3 m h x0) ∪
+           { ((NONE,x0,(q0,[])),((m.start,[]),[m.ssSym;x0])) })`
+     by METIS_TAC [FINITE_rule3, FINITE_rule2, FINITE_rule1, FINITE_UNION,
+                   FINITE_SING] THEN
+  `∃r. set r =  ((rule1 m h ∪ rule2 m h ∪ rule3 m h x0) ∪
+                { ((NONE,x0,(q0,[])),((m.start,[]),[m.ssSym;x0])) })`
+     by METIS_TAC [listExists4Set] THEN
+  `FINITE {(q,[]:(α, β) symbol list) | q ∈ m.final}`
+     by METIS_TAC [FINITE_finalStateSet] THEN
+  `∃f. set f = {(q,[]:(α, β) symbol list) | q ∈ m.final}`
+     by METIS_TAC [listExists4Set] THEN
+  Q.EXISTS_TAC `pda (q0,[]) x0 r f` THEN
+  SRW_TAC [][] THEN
+  FULL_SIMP_TAC (srw_ss()) [EXTENSION] THEN
+  METIS_TAC []
+);
+
+val invHomomorphismThm = store_thm("invHomomorphismThm",
+``∀g (h:('nts, 'ts) symbol -> ('nts, 'ts) symbol list).
+    INFINITE (UNIV:'nts set) ∧ INFINITE (UNIV:('nts,'ts) symbol set) ∧
+    INFINITE (UNIV:'state set) ∧
+    [] ∉ language (g:('nts,'ts) grammar) ⇒
+    ∃g'. language g' = inverseHomomorphism h g``,
+
+SRW_TAC [][] THEN
+`∃g'.isGnf g' ∧ (language g = language g')` by METIS_TAC [gnfExists] THEN
 `∃(m:(('nts, 'ts) symbol, ('nts, 'ts) symbol, 'state) pda).
-            x ∈ language g = x ∈ laes m` by METIS_TAC [thm5_3]
-
-
-`∃m'.hInvpda m m' h` by MAGIC
+            x ∈ language g = x ∈ laes m` by METIS_TAC [thm5_3] THEN
+`∃m'.hInvpda m m' h` by METIS_TAC [exists_hInvpda]
 
 `(x ∈ lafs m' = x ∈ { w | (FLAT (MAP h w)) ∈ lafs m })` by METIS_TAC [invhEq]
+`∃g. pda2grammar m g` by METIS_TAC [p2gGrExists]
+Q.EXISTS_TAC `g` THEN
+`x ∈ lafs m` by METIS_TAC [laes]
+
 FULL_SIMP_TAC (srw_ss()) [language_def, inverseHomomorphism, EXTENSION]
-`x ∈ lafs m` by MAGIC
-Q.EXISTS_TAC `g` 
+
+Q.EXISTS_TAC `G ...`
+
+Q.EXISTS_TAC `g`
 SRW_TAC [][]
 METIS_TAC []
-
-
-
-fun MAGIC (asl, w) = ACCEPT_TAC (mk_thm(asl,w)) (asl,w);
+hInvpda (m:(α, β, γ) pda) (m':(α, β, γ # α list) pda) (h: α -> α list)
 
 
 val _ = export_theory();
